Progress on universal PRF

src/tls/KDF.Common.fst
@@ -1,5 +1,5 @@
 (*--build-config
-options:--use_hints --fstar_home ../../../FStar --include ../../../FStar/ucontrib/Platform/fst/ --include ../../../FStar/ucontrib/CoreCrypto/fst/ --include ../../../FStar/examples/low-level/crypto/real --include ../../../FStar/examples/low-level/crypto/spartan --include ../../../FStar/examples/low-level/LowCProvider/fst --include ../../../FStar/examples/low-level/crypto --include ../../libs/ffi --include ../../../FStar/ulib/hyperstack --include ideal-flags;
+options:--fstar_home ../../../FStar --max_fuel 4 --initial_fuel 0 --max_ifuel 2 --initial_ifuel 1 --z3rlimit 20 --__temp_no_proj Handshake --__temp_no_proj Connection --use_hints --include ../../../FStar/ucontrib/CoreCrypto/fst/ --include ../../../FStar/ucontrib/Platform/fst/ --include ../../../hacl-star/secure_api/LowCProvider/fst --include ../../../kremlin/kremlib --include ../../../hacl-star/specs --include ../../../hacl-star/code/lib/kremlin --include ../../../hacl-star/code/bignum --include ../../../hacl-star/code/experimental/aesgcm --include ../../../hacl-star/code/poly1305 --include ../../../hacl-star/code/salsa-family --include ../../../hacl-star/secure_api/test --include ../../../hacl-star/secure_api/utils --include ../../../hacl-star/secure_api/vale --include ../../../hacl-star/secure_api/uf1cma --include ../../../hacl-star/secure_api/prf --include ../../../hacl-star/secure_api/aead --include ../../libs/ffi --include ../../../FStar/ulib/hyperstack --include ../../src/tls/ideal-flags;
 --*)
 (**
  Shared state for secret expansion and salt expansion
@@ -25,49 +25,114 @@ module MR = FStar.Monotonic.RRef
 module HH = FStar.HyperHeap
 module HS = FStar.HyperStack
 
+(*)
 (* Source index is a secret index *)
 type id = secretId
 
 (* The kind of expansion, either salt of expanded secret *)
 type expand_kind (i:id) =
   | ExpandSalt: expand_kind i
-  | ExpandSecret:
-     log: hashed_log ->
-     li: logInfo{
-         (EarlySecretID? i ==> LogInfo_CH? li) /\
-         (HandshakeSecretID? i ==> LogInfo_SH? li) /\
-         (ApplicationSecretID? i ==> LogInfo_SF? li) /\
-         log_info li log
-       } ->
-     expand_kind i
+  | ExpandBinder: expand_kind i
+  | ExpandBinderResumption: expand_kind i
+  | ExpandEarlyExporter: log:hashed_log -> li:logInfo{LogInfo_CH? li /\ log_info li log} -> expand_kind i
+  | ExpandEarlyTrafffic: log:hashed_log -> li:logInfo{LogInfo_CH? li /\ log_info li log} -> expand_kind i
+  | ExpandClientHandshakeTraffic: log:hashed_log -> li:logInfo{LogInfo_SH? li /\ log_info li log} -> expand_kind i
+  | ExpandServerHandshakeTraffic: log:hashed_log -> li:logInfo{LogInfo_SH? li /\ log_info li log} -> expand_kind i
+  | ExpandClientApplicationTraffic: log:hashed_log -> li:logInfo{LogInfo_SF? li /\ log_info li log} -> expand_kind i
+  | ExpandServerApplicationTraffic: log:hashed_log -> li:logInfo{LogInfo_SF? li /\ log_info li log} -> expand_kind i
+  | ExpandExporter: log:hashed_log -> li:logInfo{LogInfo_SF? li /\ log_info li log} -> expand_kind i
+  | ExpandResumption: log:hashed_log -> li:logInfo{LogInfo_CF? li /\ log_info li log} -> expand_kind i
 
 // Conceptually, this is either a KDF.Salt.X.state i or KDF.Expand.state i
 // However, the table stores actual key values, and the proper interface for
 // accessing it is spread between KDF.Salt.X and KDF.Expand
 type extracted_secret (#i:id) (x:expand_kind i) =
   lbytes (Hashing.Spec.tagLen (secretId_hash i))
+*)
 
-type expand_log (i:id) (r:rgn) =
-  (if Flags.ideal_KEF then
-    MM.t r (expand_kind i) (extracted_secret #i) (fun _ -> True)
-  else
-    unit)
+type ideal_log (dt:Type0) (rt:dt -> Tot Type0) (r:rgn) =
+  MM.t r dt rt (fun _ -> True)
+type expand_log (dt:Type0) (rt:dt -> Tot Type0) (r:rgn) =
+  (if Flags.ideal_KEF then ideal_log dt rt r else unit)
 
-type state (i:id) =
-  | State:
+abstract noeq type prf (#it:Type0) (i:it) =
+  | PRF:
     r:rgn ->
-    log: expand_log i r ->
-    state i
+    hashAlg: (it -> Tot Hashing.Spec.alg) ->
+    honest_prf: bool ->
+    key: Hashing.Spec.tag (hashAlg i) ->
+    domain: (t:Type0{hasEq t}) ->
+    range: (domain -> Tot Type0) ->
+    format: (domain -> Tot bytes) ->
+    log: expand_log domain range r ->
+    pre: (domain -> expand_log domain range r -> h:HS.mem -> GTot Type0) ->
+    post: (d:domain -> range d -> expand_log domain range r -> h0:HS.mem -> h1:HS.mem -> GTot Type0) ->
+    honestT: (p:(domain -> GTot Type0){not Flags.ideal_KEF ==> (forall (d:domain).~(p d))}) ->
+    is_honest: (d:domain -> ST bool
+      (requires fun h0 -> True)
+      (ensures fun h0 b h1 -> h0 == h1 /\ b <==> honestT d)) ->
+    gen: (d:domain -> ST (range d)
+      (requires fun h -> honestT d /\ (Flags.ideal_KEF ==> pre d log h))
+      (ensures fun h0 o h1 -> Flags.ideal_KEF ==> post d o log h0 h1)) ->
+    coerce: (d:domain -> Hashing.Spec.tag (hashAlg i) -> ST (range d)
+      (requires fun h -> ~(honestT d) /\ (Flags.ideal_KEF ==> pre d log h))
+      (ensures fun h0 o h1 -> Flags.ideal_KEF ==> post d o log h0 h1)) ->
+    prf #it i
 
-let kdf_region:rgn = new_region tls_tables_region
-type kdf_instance_table =
-  (if Flags.ideal_KEF then
-    MM.t kdf_region id state (fun _ -> True)
-  else
-    unit)
+// Create an honest PRF instance at index i of type it
+let create (#it:Type0) (i:it) (r:rgn) (hashAlg: it -> Tot Hashing.Spec.alg)
+  (domain:Type0{hasEq t}) (range:domain -> Tot Type0) (format: domain -> Tot bytes)
+  (pre: domain -> expand_log domain range r -> h:HS.mem -> GTot Type0)
+  (post: d:domain -> range d -> expand_log domain range r -> h0:HS.mem -> h1:HS.mem -> GTot Type0)
+  (honestT: p:(domain -> GTot Type0){not Flags.ideal_KEF ==> (forall (d:domain).~(p d))})
+  : ST (prf #it i)
+  (requires fun h0 -> True)
+  (ensures fun h0 _ h1 -> h0 == h1)
+  =
+  admit()
 
-let kdf_instances : kdf_instance_table =
-  (if Flags.ideal_KEF then
-    MM.alloc #kdf_region #id #state #(fun _ -> True)
+
+let random (len:nat) : ST (lbytes len)
+  (requires fun h0 -> True) (ensures fun h0 _ h1 -> h0 == h1)
+  = assume false; CoreCrypto.random len
+
+#set-options "--z3rlimit 100 --initial_fuel 2 --max_fuel 2 --initial_ifuel 2 --max_ifuel 2"
+let expand (#it:Type0) (#i:it) (prf:prf #it i) (input:PRF?.domain prf)
+  : ST (output: (PRF?.range prf) input)
+  (requires (fun h0 ->
+    Flags.ideal_KEF ==> (PRF?.pre prf) input (PRF?.log prf) h0))
+  (ensures (fun h0 r h1 -> True))
+  =
+  let ha = (PRF?.hashAlg prf) i in
+  if Flags.ideal_KEF then
+    let h0 = ST.get() in
+    cut((PRF?.pre prf) input (PRF?.log prf) h0);
+    let log : ideal_log (PRF?.domain prf) (PRF?.range prf) (PRF?.r prf) = PRF?.log prf in
+    MR.m_recall log;
+    match MM.lookup log input with
+    | Some v -> v
+    | None ->
+      cut(MM.sel (MR.m_sel h0 log) input == None);
+      let h1 = ST.get() in
+      cut(h0 == h1);
+      let key =
+        if PRF?.honest_prf prf then random (Hashing.Spec.tagLen ha)
+        else HKDF.hkdf_expand ha (PRF?.key prf) ((PRF?.format prf) input) (Hashing.Spec.tagLen ha) in
+      let h2 = ST.get() in
+      assume(h2 == h1);
+      cut((PRF?.pre prf) input (PRF?.log prf) h2);
+      let h5 = ST.get () in
+      let b = (PRF?.is_honest prf) input in
+      let h3 = ST.get() in
+      assume (h3 == h5); // Why?
+      let output =
+        if b then (PRF?.gen prf) input
+        else (PRF?.coerce prf) input key in
+      let h4 = ST.get() in
+      assume(h0 == h4);
+      cut(MM.sel (MR.m_sel h4 log) input == None);
+      MM.extend log input output;
+      output
   else
-    ())
+    let k = HKDF.hkdf_expand ha (PRF?.key prf) ((PRF?.format prf) input) (Hashing.Spec.tagLen ha) in
+    (PRF?.coerce prf) input k
